wip on sem_block_absent

SyBloc/SBSyntax.v
@@ -3,6 +3,7 @@ Require Import Velus.Operators.
 Require Import Velus.NLustre.NLExprSyntax.
 Require Import Velus.Clocks.
 
+Require Import Permutation.
 Require Import List.
 Import List.ListNotations.
 Open Scope list_scope.
@@ -28,7 +29,7 @@ Module Type SBSYNTAX
       forall x ck e,
         Is_last_in_eq x (EqNext x ck e).
 
-  Definition Is_last_in_eqs (x: ident) (eqs: list equation) : Prop :=
+  Definition Is_last_in (x: ident) (eqs: list equation) : Prop :=
     Exists (Is_last_in_eq x) eqs.
 
   Inductive Is_block_in_eq : ident -> equation -> Prop :=
@@ -54,7 +55,7 @@ Module Type SBSYNTAX
         In x xs ->
         Is_defined_in_eq x (EqCall s xs ck rst b es).
 
-  Definition Is_defined_in_eqs (x: ident) (eqs: list equation) : Prop :=
+  Definition Is_defined_in (x: ident) (eqs: list equation) : Prop :=
     Exists (Is_defined_in_eq x) eqs.
 
   Inductive Is_variable_in_eq: ident -> equation -> Prop :=
@@ -66,7 +67,7 @@ Module Type SBSYNTAX
         In x xs ->
         Is_variable_in_eq x (EqCall s xs ck rst b es).
 
-  Definition Is_variable_in_eqs (x: ident) (eqs: list equation) : Prop :=
+  Definition Is_variable_in (x: ident) (eqs: list equation) : Prop :=
     Exists (Is_variable_in_eq x) eqs.
 
   Inductive Is_state_in_eq: ident -> nat -> equation -> Prop :=
@@ -77,12 +78,68 @@ Module Type SBSYNTAX
       forall s xs ck rst b es,
         Is_state_in_eq s 1 (EqCall s xs ck rst b es).
 
-  Definition Is_state_in_eqs (s: ident) (k: nat) (eqs: list equation) : Prop :=
+  Definition Is_state_in (s: ident) (k: nat) (eqs: list equation) : Prop :=
     Exists (Is_state_in_eq s k) eqs.
 
-  Definition Reset_in (s: ident) := Is_state_in_eqs s 0.
+  Definition Reset_in (s: ident) := Is_state_in s 0.
 
-  Definition Step_in (s: ident) := Is_state_in_eqs s 1.
+  Definition Step_in (s: ident) := Is_state_in s 1.
+
+  Fixpoint lasts_of (eqs: list equation) : list ident :=
+    match eqs with
+    | [] => []
+    | EqNext x _ _ :: eqs => x :: (lasts_of eqs)
+    | _ :: eqs => lasts_of eqs
+    end.
+
+  Lemma lasts_of_in:
+    forall eqs x,
+      Is_last_in x eqs <-> In x (lasts_of eqs).
+  Proof.
+    induction eqs as [|[]]; simpl.
+    - now setoid_rewrite Exists_nil.
+    - setoid_rewrite <-IHeqs; split; try right; auto.
+      inversion_clear 1 as [?? Last|]; try inv Last; auto.
+    - setoid_rewrite <-IHeqs; split.
+      + inversion_clear 1 as [?? Last|]; try inv Last; auto.
+      + intros [E|?].
+        * subst; left; constructor.
+        * right; auto.
+    - setoid_rewrite <-IHeqs; split; try right; auto.
+      inversion_clear 1 as [?? Last|]; try inv Last; auto.
+    - setoid_rewrite <-IHeqs; split; try right; auto.
+      inversion_clear 1 as [?? Last|]; try inv Last; auto.
+  Qed.
+
+  Fixpoint states_of (eqs: list equation) : list ident :=
+    match eqs with
+    | [] => []
+    | EqReset s _ _ :: eqs => s :: states_of eqs
+    | EqCall s _ _ _ _ _ :: eqs => s :: states_of eqs
+    | _ :: eqs => states_of eqs
+    end.
+
+  Lemma states_of_in:
+    forall eqs s,
+      (exists k, Is_state_in s k eqs) <-> In s (states_of eqs).
+  Proof.
+    induction eqs as [|[]]; simpl.
+    - setoid_rewrite Exists_nil; split; try contradiction; intros ** (); eauto.
+    - setoid_rewrite <-IHeqs; split; intros ** (); try (eexists; right; eauto).
+      inversion_clear 1 as [?? Block|]; try inv Block; eauto.
+    - setoid_rewrite <-IHeqs; split; intros ** (); try (eexists; right; eauto).
+      inversion_clear 1 as [?? Block|]; try inv Block; eauto.
+    - setoid_rewrite <-IHeqs; split.
+      + intros ** (); inversion_clear 1 as [?? Block|]; try inv Block; eauto.
+      + intros [E|(?&?)].
+        * subst; eexists; left; constructor.
+        * eexists; right; eauto.
+    - setoid_rewrite <-IHeqs; split.
+      + intros ** (); inversion_clear 1 as [?? Block|]; try inv Block; eauto.
+      + intros [E|(?&?)].
+        * subst; eexists; left; constructor.
+        * eexists; right; eauto.
+  Qed.
 
   Record block :=
     Block {
@@ -100,11 +157,13 @@ Module Type SBSYNTAX
         b_nodup_lasts_blocks: NoDup (map fst b_lasts ++ map fst b_blocks);
 
         b_blocks_in_eqs: forall f, (exists i, In (i, f) b_blocks) <-> Is_block_in f b_eqs;
-        b_lasts_in_eqs: forall x, InMembers x b_lasts <-> Is_last_in_eqs x b_eqs;
-        b_vars_out_in_eqs: forall x, InMembers x (b_vars ++ b_out) <-> Is_variable_in_eqs x b_eqs;
+        (* b_lasts_in_eqs: forall x, InMembers x b_lasts <-> Is_last_in_eqs x b_eqs; *)
+        b_lasts_in_eqs: Permutation (map fst b_lasts) (lasts_of b_eqs);
+        b_vars_out_in_eqs: forall x, InMembers x (b_vars ++ b_out) <-> Is_variable_in x b_eqs;
         (* b_out_not_last: forall x, InMembers x b_out -> ~ Is_last_in_eqs x b_eqs; *)
 
-        b_states_in_eqs: forall s, InMembers s b_blocks <-> (exists k, Is_state_in_eqs s k b_eqs);
+        (* b_states_in_eqs: forall s, InMembers s b_blocks <-> (exists k, Is_state_in s k b_eqs); *)
+        b_states_in_eqs: Permutation (map fst b_blocks) (states_of b_eqs);
 
         b_no_single_reset: forall s, Reset_in s b_eqs -> Step_in s b_eqs;
 
@@ -122,12 +181,28 @@ Module Type SBSYNTAX
     apply NoDup_comm, NoDup_app_weaken, NoDup_app_weaken in Nodup; auto.
   Qed.
 
+  Lemma b_nodup_lasts_of:
+    forall b, NoDup (lasts_of b.(b_eqs)).
+  Proof.
+    setoid_rewrite <-b_lasts_in_eqs;
+      setoid_rewrite <-fst_NoDupMembers.
+    apply b_nodup_lasts.
+  Qed.
+
   Lemma b_nodup_blocks:
     forall b, NoDupMembers b.(b_blocks).
   Proof.
     intro; pose proof (b_nodup_lasts_blocks b) as Nodup.
     apply NoDup_comm, NoDup_app_weaken in Nodup.
     apply fst_NoDupMembers; auto.
+  Qed.
+
+  Lemma b_nodup_states_of:
+    forall b, NoDup (states_of b.(b_eqs)).
+  Proof.
+    setoid_rewrite <-b_states_in_eqs;
+      setoid_rewrite <-fst_NoDupMembers.
+    apply b_nodup_blocks.
   Qed.
 
   Lemma b_nodup_vars:
@@ -143,10 +218,10 @@ Module Type SBSYNTAX
     apply fst_NoDupMembers; auto.
   Qed.
 
-  Lemma Is_defined_Is_variable_Is_last_in_eqs:
+  Lemma Is_defined_Is_variable_Is_last_in:
     forall eqs x,
-      Is_defined_in_eqs x eqs ->
-      Is_variable_in_eqs x eqs \/ Is_last_in_eqs x eqs.
+      Is_defined_in x eqs ->
+      Is_variable_in x eqs \/ Is_last_in x eqs.
   Proof.
     induction eqs; inversion_clear 1 as [?? Def|?? Defs].
     - inv Def.
@@ -161,17 +236,16 @@ Module Type SBSYNTAX
   Lemma b_ins_not_def:
     forall b x,
       InMembers x b.(b_in) ->
-      ~ Is_defined_in_eqs x b.(b_eqs).
+      ~ Is_defined_in x b.(b_eqs).
   Proof.
     intros ** Hin Hdef.
     pose proof (b_nodup b) as Nodup.
     eapply (NoDup_app_In x) in Nodup.
-    - apply Is_defined_Is_variable_Is_last_in_eqs in Hdef as [Var|Last];
+    - apply Is_defined_Is_variable_Is_last_in in Hdef as [Var|Last];
         apply Nodup, in_app.
       + apply b_vars_out_in_eqs in Var.
         right; rewrite <-map_app; apply fst_InMembers; auto.
-      + apply b_lasts_in_eqs in Last.
-        left; apply fst_InMembers; auto.
+      + apply lasts_of_in in Last; rewrite <-b_lasts_in_eqs in Last; auto.
     - apply fst_InMembers; auto.
   Qed.
 
@@ -330,6 +404,33 @@ Module Type SBSYNTAX
     split; intro HH.
     - split; intro; apply HH; unfold Is_block_in; intuition.
     - destruct HH; inversion_clear 1; intuition.
+  Qed.
+
+  Lemma not_Is_last_in_cons:
+    forall x eq eqs,
+      ~ Is_last_in x (eq :: eqs) <-> ~ Is_last_in_eq x eq /\ ~ Is_last_in x eqs.
+  Proof.
+    split; intros HH.
+    - split; intro; apply HH; unfold Is_last_in; intuition.
+    - destruct HH; inversion_clear 1; intuition.
+  Qed.
+
+  Lemma not_Is_state_in_cons:
+    forall s k eq eqs,
+      ~ Is_state_in s k (eq :: eqs) <-> ~ Is_state_in_eq s k eq /\ ~ Is_state_in s k eqs.
+  Proof.
+    split; intros HH.
+    - split; intro; apply HH; unfold Is_state_in; intuition.
+    - destruct HH; inversion_clear 1; intuition.
+  Qed.
+
+  Lemma not_Is_state_in_cons':
+    forall s eq eqs,
+      (forall k, ~ Is_state_in s k (eq :: eqs)) <-> (forall k, ~ Is_state_in_eq s k eq) /\ (forall k, ~ Is_state_in s k eqs).
+  Proof.
+    split; intros HH.
+    - split; intros ? ?; eapply HH; unfold Is_state_in; eauto.
+    - intro; destruct HH; inversion_clear 1; intuition; eauto.
   Qed.
 
 End SBSYNTAX.
